update： pl/MonadHoare.v

pl/MonadHoare.v
@@ -3,7 +3,8 @@ Require Import Coq.Strings.String.
 Require Import Coq.ZArith.ZArith.
 Require Import Coq.micromega.Psatz.
 Require Import Coq.Classes.Morphisms.
-Require Import Coq.Lists.List.
+Require Import Coq.Sorting.Permutation.
+Require Import Coq.Lists.List. Import ListNotations.
 Require Import SetsClass.SetsClass. Import SetsNotation.
 Require Import PL.Syntax.
 Require Import PL.DenotationsOfExpr.
@@ -176,6 +177,8 @@ Qed.
 
 (** * 霍尔逻辑证明 *)
 
+(** ** 3x + 1 *)
+
 Theorem functional_correctness_3x1:
   forall n: Z,
     n >= 1 ->
@@ -201,6 +204,8 @@ Proof.
     apply Hoare_ret.
     lia.
 Qed.
+
+(** ** 二分查找 *)
 
 Theorem functional_correctness_binary_search:
   forall (P: Z -> Prop) lo hi,
@@ -230,4 +235,347 @@ Proof.
       tauto.
 Qed.
 
+(** ** 归并 *)
+
+Local Close Scope sets.
+Local Open Scope list.
+
+Fixpoint incr_aux (l: list Z) (x: Z): Prop :=
+  match l with
+  | nil => True
+  | y :: l0 => x <= y /\ incr_aux l0 y
+  end.
+
+Definition incr (l: list Z): Prop :=
+  match l with
+  | nil => True
+  | x :: l0 => incr_aux l0 x
+  end.
+
+Lemma incr_app_cons: forall l1 x l2,
+  incr (l1 ++ [x]) ->
+  incr (x :: l2) ->
+  incr (l1 ++ x :: l2).
+Proof.
+  intros.
+  simpl in H0.
+  destruct l1 as [| a l1]; simpl in *.
+  { tauto. }
+  revert a H; induction l1; simpl; intros.
+  + tauto.
+  + split; [tauto |].
+    apply IHl1.
+    tauto.
+Qed.
+
+Lemma incr_app_cons_inv1: forall l1 x l2,
+  incr (l1 ++ x :: l2) ->
+  incr (l1 ++ [x]).
+Proof.
+  intros.
+  destruct l1 as [| a l1]; simpl in *.
+  { tauto. }
+  revert a H; induction l1; simpl; intros.
+  + tauto.
+  + split; [tauto |].
+    apply IHl1.
+    tauto.
+Qed.
+
+Lemma incr_app_cons_inv2: forall l1 x l2,
+  incr (l1 ++ x :: l2) ->
+  incr (x :: l2).
+Proof.
+  intros.
+  simpl.
+  induction l1; simpl in *.
+  + tauto.
+  + apply IHl1.
+    destruct l1; simpl in *; tauto.
+Qed.
+
+Theorem merge_perm:
+  forall l1 l2,
+    Hoare (merge l1 l2) (Permutation (l1 ++ l2)).
+Proof.
+  intros.
+  unfold merge.
+  apply (Hoare_repeat_break _
+           (fun '(l1', l2', l3') =>
+              Permutation (l1 ++ l2) (l1' ++ l2' ++ l3'))).
+  2: {
+    rewrite app_nil_r.
+    reflexivity.
+  }
+  intros [[l1' l2'] l3'] ?.
+  unfold body_merge.
+  destruct l1' as [ | x l1']; [| destruct l2' as [| y l2']].
+  + apply Hoare_ret.
+    rewrite H; simpl.
+    apply Permutation_app_comm.
+  + apply Hoare_ret.
+    rewrite H.
+    rewrite Permutation_app_comm.
+    reflexivity.
+  + apply Hoare_choice; apply Hoare_assume_bind; intros.
+    - apply Hoare_ret.
+      rewrite H.
+      rewrite ! app_assoc.
+      rewrite (Permutation_app_comm _ [x]).
+      reflexivity.
+    - apply Hoare_ret.
+      rewrite H.
+      apply Permutation_app; [reflexivity |].
+      rewrite ! app_assoc.
+      rewrite (Permutation_app_comm _ [y]).
+      reflexivity.
+Qed.
+
+Theorem merge_incr:
+  forall l1 l2,
+    incr l1 ->
+    incr l2 ->
+    Hoare (merge l1 l2) incr.
+Proof.
+  intros.
+  unfold merge.
+  apply (Hoare_repeat_break _
+           (fun '(l1', l2', l3') => 
+              incr (l3' ++ l1') /\
+              incr (l3' ++ l2'))).
+  2: {
+    tauto.
+  }
+  clear l1 l2 H H0.
+  intros [[l1 l2] l3] [? ?].
+  destruct l1 as [ | x l1]; [| destruct l2 as [| y l2]].
+  + apply Hoare_ret; tauto.
+  + apply Hoare_ret; tauto.
+  + apply Hoare_choice; apply Hoare_assume_bind; intros.
+    - apply Hoare_ret.
+      split.
+      * rewrite <- app_assoc.
+        exact H.
+      * rewrite <- app_assoc.
+        simpl.
+        apply incr_app_cons_inv1 in H.
+        apply incr_app_cons_inv2 in H0.
+        apply incr_app_cons; simpl in *; tauto.
+    - apply Hoare_ret.
+      split.
+      * rewrite <- app_assoc.
+        simpl.
+        apply incr_app_cons_inv1 in H0.
+        apply incr_app_cons_inv2 in H.
+        apply incr_app_cons; simpl in *; tauto.
+      * rewrite <- app_assoc.
+        exact H0.
+Qed.
+
+Theorem functional_correctness_merge:
+  forall l1 l2,
+    incr l1 ->
+    incr l2 ->
+    Hoare (merge l1 l2)
+          (fun l3 => Permutation (l1 ++ l2) l3 /\ incr l3).
+Proof.
+  intros.
+  apply Hoare_conjunct.
+  + apply merge_perm.
+  + apply merge_incr; tauto.
+Qed.
+
+(** ** 拓展欧几里得 *)
+
+Local Close Scope list.
+Local Open Scope sets.
+
+Definition any (A: Type): SetMonad.M A := Sets.full.
+
+Definition body_ext_euclid
+             (W: Z -> Z -> SetMonad.M (Z * Z))
+             (a b: Z): SetMonad.M (Z * Z) :=
+  choice
+    (assume (b = 0);; 
+     choice
+       (assume (a >= 0);; ret (1, 0))
+       (assume (a <= 0);; ret (-1, 0)))
+    (assume (b <> 0);;
+     q <- any Z;;
+     r <- any Z;;
+     assume (a = r + q * b);;
+     '(x, y) <- W b r;;
+     ret (y, x - q * y)).
+
+Definition ext_euclid (a b: Z): SetMonad.M (Z * Z) :=
+  Kleene_LFix body_ext_euclid a b.
+
+
+Lemma Hoare_Kleene_LFix2 {A1 A2 B: Type}:
+  forall (a1: A1) (a2: A2)
+         (Q: B -> Prop)
+         (f: (A1 -> A2 -> SetMonad.M B) ->
+             (A1 -> A2 -> SetMonad.M B)),
+    (forall n, Hoare (Nat.iter n f ∅ a1 a2) Q) ->
+    Hoare (Kleene_LFix f a1 a2) Q.
+Proof.
+  intros.
+  unfold Hoare.
+  intros b HFix.
+  change (b ∈ (⋃ (fun n => Nat.iter n f ∅ a1 a2))) in HFix.
+  change (exists n, b ∈ Nat.iter n f ∅ a1 a2) in HFix.
+  destruct HFix as [n ?].
+  unfold Hoare in H.
+  pose proof H n b H0.
+  tauto.
+Qed.
+
+Theorem Hoare_any_bind {A B: Type}:
+  forall (f: A -> SetMonad.M B) (Q: B -> Prop),
+    (forall a, Hoare (f a) Q) ->
+    Hoare (bind (any A) f) Q.
+Proof.
+  intros.
+  apply (Hoare_bind _ _ (fun _ => True)).
+  + unfold Hoare, any.
+    intros. tauto.
+  + intros.
+    apply H.
+Qed.
+
+Lemma functional_correctness_ext_euclid_aux:
+  forall W,
+    (forall a b, Hoare
+                   (W a b)
+                   (fun '(x, y) => a * x + b * y = Z.gcd a b)) ->
+    (forall a b, Hoare
+                   (body_ext_euclid W a b)
+                   (fun '(x, y) => a * x + b * y = Z.gcd a b)).
+Proof.
+  intros.
+  unfold body_ext_euclid.
+  apply Hoare_choice.
+  + apply Hoare_assume_bind.
+    intros.
+    apply Hoare_choice.
+    - apply Hoare_assume_bind.
+      intros.
+      apply Hoare_ret.
+      rewrite H0.
+      rewrite Z.gcd_0_r.
+      lia.
+    - apply Hoare_assume_bind.
+      intros.
+      apply Hoare_ret.
+      rewrite H0.
+      rewrite Z.gcd_0_r.
+      lia.
+  + apply Hoare_assume_bind.
+    intros.
+    apply Hoare_any_bind.
+    intros q.
+    apply Hoare_any_bind.
+    intros r.
+    apply Hoare_assume_bind.
+    intros.
+    eapply Hoare_bind.
+    1: { apply H. }
+    intros [y x] ?.
+    apply Hoare_ret.
+    pose proof Z.gcd_comm a b.
+    pose proof Z.gcd_add_mult_diag_r b r q.
+    rewrite <- H1 in H4.
+    nia.
+Qed.
+
+Theorem functional_correctness_ext_euclid:
+  forall a b,
+    Hoare (ext_euclid a b)
+          (fun '(x, y) => a * x + b * y = Z.gcd a b).
+Proof.
+  intros.
+  revert a b.
+  unfold ext_euclid.
+  intros.
+  apply Hoare_Kleene_LFix2.
+  intros n.
+  revert a b.
+  induction n; simpl; intros.
+  + unfold Hoare; sets_unfold; intros; tauto.
+  + apply functional_correctness_ext_euclid_aux.
+    apply IHn.
+Qed.
+
+(** ** 归并排序 *)
+
+Local Open Scope list.
+
+Definition ext_sort (l: list Z): SetMonad.M (list Z) :=
+  fun l' => Permutation l l' /\ incr l'.
+
+Definition ext_split (l: list Z): SetMonad.M (list Z * list Z) :=
+  fun '(l0, l1) => Permutation l (l0 ++ l1).
+
+Definition gmergesort_f (W: list Z -> SetMonad.M (list Z)):
+  list Z -> SetMonad.M (list Z) :=
+  fun x => 
+    choice
+      (ext_sort x)
+      (assume(length x >= 2)%nat;;
+       '(p1, q1) <- ext_split x ;; 
+       p2 <- W (p1) ;; 
+       q2 <- W (q1) ;; 
+       merge p2 q2).
+
+Definition gmergesort := Kleene_LFix gmergesort_f.
+Lemma ext_sort_fact:
+  forall l,
+    Hoare (ext_sort l) (fun l0 => Permutation l l0 /\ incr l0).
+Proof.
+  unfold Hoare, ext_sort; sets_unfold.
+  intros.
+  tauto.
+Qed.
+
+Lemma ext_split_fact:
+  forall l,
+    Hoare (ext_split l) (fun '(l1, l2) => Permutation l (l1 ++ l2)).
+Proof.
+  unfold Hoare, ext_split; sets_unfold.
+  intros.
+  tauto.
+Qed.
+
+Theorem functional_correctness_mergesort:
+  forall l,
+    Hoare (gmergesort l) (fun l0 => Permutation l l0 /\ incr l0).
+Proof.
+  intros.
+  unfold Hoare, gmergesort, Kleene_LFix; unfold_CPO_defs.
+  intros.
+  destruct H as [n ?].
+  revert l a H.
+  change (forall l,
+          Hoare (Nat.iter n gmergesort_f ∅ l)
+                (fun l0 => Permutation l l0 /\ incr l0)).
+  induction n; simpl; intros.
+  + unfold Hoare; sets_unfold; intros; tauto.
+  + unfold gmergesort_f at 1.
+    apply Hoare_choice; [apply ext_sort_fact |].
+    apply Hoare_assume_bind.
+    intros.
+    eapply Hoare_bind; [apply ext_split_fact |].
+    intros [l1 l2] ?.
+    eapply Hoare_bind; [apply IHn |].
+    intros l1' [? ?].
+    eapply Hoare_bind; [apply IHn |].
+    intros l2' [? ?].
+    eapply Hoare_conseq; [| apply functional_correctness_merge; tauto].
+    intros l3 [? ?].
+    rewrite <- H5 at 1.
+    rewrite <- H1, <- H3.
+    tauto.
+Qed.
+
 End SetMonadHoare.
+
